theories/ftlr/Jnz.v
@@ -7,36 +7,28 @@ From cap_machine.rules Require Import rules_base rules_Jnz.
 
 Section fundamental.
   Context {Σ:gFunctors} {memg:memG Σ} {regg:regG Σ}
-          {stsg : STSG Addr region_type Σ} {heapg : heapG Σ}
-          `{MonRef: MonRefG (leibnizO _) CapR_rtc Σ} {nainv: logrel_na_invs Σ}
+          {nainv: logrel_na_invs Σ}
           `{MachineParameters}.
 
-  Notation STS := (leibnizO (STS_states * STS_rels)).
-  Notation STS_STD := (leibnizO (STS_std_states Addr region_type)).
-  Notation WORLD := (prodO STS_STD STS). 
-  Implicit Types W : WORLD.
-
-  Notation D := (WORLD -n> (leibnizO Word) -n> iProp Σ).
-  Notation R := (WORLD -n> (leibnizO Reg) -n> iProp Σ).
+  Notation D := ((leibnizO Word) -n> iProp Σ).
+  Notation R := ((leibnizO Reg) -n> iProp Σ).
   Implicit Types w : (leibnizO Word).
   Implicit Types interp : (D).
   
   (* TODO: Move somewhere *)
   Ltac destruct_cap c :=
     let p := fresh "p" in
-    let g := fresh "g" in
     let b := fresh "b" in
     let e := fresh "e" in
     let a := fresh "a" in
-    destruct c as ((((p & g) & b) & e) & a).
+    destruct c as (((p & b) & e) & a).
 
-  Lemma jnz_case (W : WORLD) (r : leibnizO Reg) (p p' : Perm)
-        (g : Locality) (b e a : Addr) (w : Word) (ρ : region_type) (r1 r2 : RegName):
-    ftlr_instr W r p p' g b e a w (Jnz r1 r2) ρ.
+  Lemma jnz_case (r : leibnizO Reg) (p : Perm)
+        (b e a : Addr) (w : Word) (r1 r2 : RegName) (P : D):
+    ftlr_instr r p b e a w (Jnz r1 r2) P.
   Proof.
-    intros Hp Hsome i Hbae Hfp Hpwl Hregion [Hnotrevoked Hnotstatic] HO Hi.
-    iIntros "#IH #Hinv #Hreg #Hinva Hmono #Hw Hsts Hown".
-    iIntros "Hr Hstate Ha HPC Hmap".
+    intros Hp Hsome i Hbae Hi.
+    iIntros "#IH #Hinv #Hinva #Hreg #Hread Hown Ha HP Hcls HPC Hmap".
     rewrite delete_insert_delete.
     iDestruct ((big_sepM_delete _ _ PC) with "[HPC Hmap]") as "Hmap /=";
       [apply lookup_insert|rewrite delete_insert_delete;iFrame|]. simpl.
@@ -47,66 +39,54 @@ Section fundamental.
 
     iIntros "!>" (regs' retv). iDestruct 1 as (HSpec) "[Ha Hmap]".
     destruct HSpec.
-    { iApply wp_pure_step_later; auto. iNext.
+    { iApply wp_pure_step_later; auto.
+      iMod ("Hcls" with "[Ha HP]");[iExists w;iFrame|iModIntro]. iNext.
       iApply wp_value; auto. iIntros; discriminate. }
     { match goal with
-      | H: incrementPC _ = Some _ |- _ => apply incrementPC_Some_inv in H as (p''&g''&b''&e''&a''& ? & HPC & Z & Hregs')
+      | H: incrementPC _ = Some _ |- _ => apply incrementPC_Some_inv in H as (p''&b''&e''&a''& ? & HPC & Z & Hregs')
       end. simplify_map_eq. rewrite insert_insert.
-      iApply wp_pure_step_later; auto. iNext.
-      iDestruct (region_close with "[$Hstate $Hr $Ha $Hmono]") as "Hr"; eauto.
-      { destruct ρ;auto;[..|specialize (Hnotstatic g)]; try contradiction. }
-      iApply ("IH" $! _ r with "[%] [] [Hmap] [$Hr] [$Hsts] [$Hown]"); try iClear "IH"; eauto. }
+      iApply wp_pure_step_later; auto. iMod ("Hcls" with "[Ha HP]");[iExists w;iFrame|iModIntro]. iNext.
+      iApply ("IH" $! r with "[%] [] [Hmap] [$Hown]"); try iClear "IH"; eauto. iAlways.
+      rewrite !fixpoint_interp1_eq /=.
+      destruct Hp as [-> | ->];iFrame "Hinv". }
     { simplify_map_eq. iApply wp_pure_step_later; auto.
       rewrite !insert_insert.
       destruct (updatePcPerm w') as [n0|c0] eqn:Hw.
       { iApply (wp_bind (fill [SeqCtx])).
         iDestruct ((big_sepM_delete _ _ PC) with "Hmap") as "[HPC Hmap]"; [apply lookup_insert|].
         iApply (wp_notCorrectPC with "HPC"); [intro; match goal with H: isCorrectPC (inl _) |- _ => inv H end|].
+        iMod ("Hcls" with "[Ha HP]");[iExists w;iFrame|iModIntro].
         iNext. iNext. iIntros "HPC /=".
         iApply wp_pure_step_later; auto.
         iApply wp_value.
         iNext. iIntros. discriminate. }
       { destruct_cap c0. destruct (PermFlowsTo RX p0) eqn:Hpft.
         { destruct w'; simpl in Hw; try discriminate.
-          destruct_cap c. assert (Heq: (if perm_eq_dec p0 p1 then True else p0 = RX /\ p1 = E) /\ g0 = g1 /\ b0 = b1 /\ e0 = e1 /\ a0 = a1) by (destruct (perm_eq_dec p0 p1); destruct p1; inv Hw; simpl in Hpft; try congruence; auto; repeat split; auto).
-          clear Hw. destruct (perm_eq_dec p0 p1); [subst p1; destruct Heq as (_ & -> & -> & -> & ->)| destruct Heq as ((-> & ->) & -> & -> & -> & ->)].
-          { iDestruct (region_close with "[$Hstate $Hr $Ha $Hmono]") as "Hr"; eauto.
-             { destruct ρ;auto;[..|specialize (Hnotstatic g0)];contradiction. }
-            iApply ("IH" $! _ r with "[%] [] [Hmap] [$Hr] [$Hsts] [$Hown]"); try iClear "IH"; eauto.
+          destruct_cap c. assert (Heq: (if perm_eq_dec p0 p1 then True else p0 = RX /\ p1 = E) /\ b0 = b1 /\ e0 = e1 /\ a0 = a1) by (destruct (perm_eq_dec p0 p1); destruct p1; inv Hw; simpl in Hpft; try congruence; auto; repeat split; auto).
+          clear Hw. destruct (perm_eq_dec p0 p1); [subst p1; destruct Heq as (_ & -> & -> & ->)| destruct Heq as ((-> & ->) & -> & -> & ->)].
+          { iMod ("Hcls" with "[Ha HP]");[iExists w;iFrame|iModIntro]. 
+            iApply ("IH" $! r with "[%] [] [Hmap] [$Hown]"); try iClear "IH"; eauto.
             - destruct p0; simpl in Hpft; auto; try discriminate.
-              destruct (reg_eq_dec r1 PC).
-              + subst r1. simplify_map_eq; auto.
-              + simplify_map_eq.
-                iDestruct ("Hreg" $! r1 n) as "Hr1".
-                rewrite /RegLocate H1. rewrite (fixpoint_interp1_eq _ (inr _)).
-                simpl; destruct g1; auto.
             - destruct (reg_eq_dec r1 PC).
               + subst r1. simplify_map_eq. auto.
               + simplify_map_eq.
                 iDestruct ("Hreg" $! r1 n) as "Hr1".
-                rewrite /RegLocate H1. rewrite (fixpoint_interp1_eq _ (inr _)).
-                destruct p0; simpl in *; try discriminate; eauto.
-                destruct g1; auto; iDestruct "Hr1" as (p0) "[HA HB]"; eauto. }
+                rewrite /RegLocate H1. rewrite !fixpoint_interp1_eq.
+                destruct p0; simpl in *; try discriminate; eauto. }
           { assert (r1 <> PC) as HPCnr1.
             { intro; subst r1; simplify_map_eq. naive_solver. }
             simplify_map_eq. iDestruct ("Hreg" $! r1 HPCnr1) as "Hr1".
-            rewrite /RegLocate H1. rewrite (fixpoint_interp1_eq _ (inr _)) /=.
-            iDestruct (region_close with "[$Hstate $Hr $Ha $Hmono]") as "Hr"; eauto.
-            { destruct ρ;auto;[..|specialize (Hnotstatic g0)];contradiction. }
-            rewrite /enter_cond.
+            rewrite /RegLocate H1. rewrite !fixpoint_interp1_eq /=.
+            iMod ("Hcls" with "[Ha HP]");[iExists w;iFrame|iModIntro]. 
             rewrite /interp_expr /=.
             iDestruct "Hr1" as "#H".
-            iAssert (future_world g1 W W) as "Hfuture".
-            { destruct g1; iPureIntro.
-              - destruct W. apply related_sts_priv_refl_world.
-              - destruct W. apply related_sts_pub_refl_world. }
-            iSpecialize ("H" $! _ _ with "Hfuture").
-            iNext. iDestruct ("H" with "[$Hmap $Hr $Hsts $Hown]") as "[_ H]"; auto. } }
+            iNext. iDestruct ("H" with "[$Hmap $Hown]") as "[_ Hcont]"; auto. } }
         iApply (wp_bind (fill [SeqCtx])).
         iDestruct ((big_sepM_delete _ _ PC) with "Hmap") as "[HPC Hmap]"; [apply lookup_insert|].
         iApply (wp_notCorrectPC with "HPC").
         - intros HH. inv HH. naive_solver.
-        - iNext. iNext. iIntros "HPC /=".
+        - iMod ("Hcls" with "[Ha HP]");[iExists w;iFrame|iModIntro].
+          iNext. iNext. iIntros "HPC /=".
           iApply wp_pure_step_later; auto.
           iApply wp_value.
           iNext. iIntros. discriminate. } }
