theories/ftlr/Mov.v
@@ -2,32 +2,25 @@ From cap_machine Require Export logrel.
 From iris.proofmode Require Import tactics.
 From iris.program_logic Require Import weakestpre adequacy lifting.
 From stdpp Require Import base.
-From cap_machine Require Import ftlr_base monotone.
+From cap_machine Require Import ftlr_base.
 From cap_machine.rules Require Import rules_base rules_Mov.
 
 Section fundamental.
   Context {Σ:gFunctors} {memg:memG Σ} {regg:regG Σ}
-          {stsg : STSG Addr region_type Σ} {heapg : heapG Σ}
-          `{MonRef: MonRefG (leibnizO _) CapR_rtc Σ} {nainv: logrel_na_invs Σ}
+          {nainv: logrel_na_invs Σ}
           `{MachineParameters}.
 
-  Notation STS := (leibnizO (STS_states * STS_rels)).
-  Notation STS_STD := (leibnizO (STS_std_states Addr region_type)).
-  Notation WORLD := (prodO STS_STD STS). 
-  Implicit Types W : WORLD.
-
-  Notation D := (WORLD -n> (leibnizO Word) -n> iProp Σ).
-  Notation R := (WORLD -n> (leibnizO Reg) -n> iProp Σ).
+  Notation D := ((leibnizO Word) -n> iProp Σ).
+  Notation R := ((leibnizO Reg) -n> iProp Σ).
   Implicit Types w : (leibnizO Word).
   Implicit Types interp : (D).
 
-  Lemma mov_case (W : WORLD) (r : leibnizO Reg) (p p' : Perm)
-        (g : Locality) (b e a : Addr) (w : Word) (ρ : region_type) (dst : RegName) (src : Z + RegName):
-    ftlr_instr W r p p' g b e a w (Mov dst src) ρ.
+  Lemma mov_case (r : leibnizO Reg) (p : Perm)
+        (b e a : Addr) (w : Word) (dst : RegName) (src : Z + RegName) (P : D):
+    ftlr_instr r p b e a w (Mov dst src) P.
   Proof.
-    intros Hp Hsome i Hbae Hfp Hpwl Hregion [Hnotrevoked Hnotstatic] HO Hi.
-    iIntros "#IH #Hinv #Hreg #Hinva Hmono #Hw Hsts Hown".
-    iIntros "Hr Hstate Ha HPC Hmap".
+    intros Hp Hsome i Hbae Hi.
+    iIntros "#IH #Hinv #Hinva #Hreg #Hread Hown Ha HP Hcls HPC Hmap".
     rewrite delete_insert_delete.
     iDestruct ((big_sepM_delete _ _ PC) with "[HPC Hmap]") as "Hmap /=";
       [apply lookup_insert|rewrite delete_insert_delete;iFrame|]. simpl.
@@ -38,33 +31,32 @@ Section fundamental.
 
     iIntros "!>" (regs' retv). iDestruct 1 as (HSpec) "[Ha Hmap]".
     destruct HSpec; cycle 1.
-    { iApply wp_pure_step_later; auto. iNext.
+    { iApply wp_pure_step_later; auto.
+      iMod ("Hcls" with "[Ha HP]"); [iExists w; iFrame|iModIntro]. iNext.
       iApply wp_value; auto. iIntros; discriminate. }
     { (* TODO: it might be possible to refactor the proof below by using more simplify_map_eq *)
       (* TODO: use incrementPC_inv *)
       match goal with
-      | H: incrementPC _ = Some _ |- _ => apply incrementPC_Some_inv in H as (p''&g''&b''&e''&a''& ? & HPC & Z & Hregs')
+      | H: incrementPC _ = Some _ |- _ => apply incrementPC_Some_inv in H as (p''&b''&e''&a''& ? & HPC & Z & Hregs')
       end. simplify_map_eq.
-      iApply wp_pure_step_later; auto. iNext.
+      iApply wp_pure_step_later; auto.
+      iMod ("Hcls" with "[Ha HP]"); [iExists w; iFrame|iModIntro].
+      iNext.
       destruct (reg_eq_dec dst PC).
       { subst dst. rewrite lookup_insert in HPC. inv HPC.
         repeat rewrite insert_insert.
         destruct src; simpl in *; try discriminate.
-        iDestruct (region_close with "[$Hstate $Hr $Ha $Hmono]") as "Hr"; eauto.
-        { destruct ρ;auto;[..|specialize (Hnotstatic g0)];contradiction. }
         destruct (reg_eq_dec PC r0).
         { subst r0. simplify_map_eq.
-          iApply ("IH" $! _ r with "[%] [] [Hmap] [$Hr] [$Hsts] [$Hown]"); try iClear "IH"; eauto. }
+          iApply ("IH" $! r with "[%] [] [Hmap] [$Hown]"); try iClear "IH"; eauto.
+          iAlways. rewrite !fixpoint_interp1_eq /=. destruct Hp as [-> | ->]; iFrame "Hinv". }
         { simplify_map_eq.
           rewrite /RegLocate. iDestruct ("Hreg" $! r0 ltac:(auto)) as "Hr0". rewrite H0.
           destruct (PermFlowsTo RX p'') eqn:Hpft.
-          - iApply ("IH" $! _ r with "[%] [] [Hmap] [$Hr] [$Hsts] [$Hown]"); try iClear "IH"; eauto.
+          - iApply ("IH" $! r with "[%] [] [Hmap] [$Hown]"); try iClear "IH"; eauto.
             + destruct p''; simpl in Hpft; auto.
-              repeat rewrite fixpoint_interp1_eq. simpl.
-              destruct g''; auto. 
             + iModIntro.
               destruct p''; simpl in Hpft; try discriminate; repeat (rewrite fixpoint_interp1_eq); simpl; auto.
-              destruct g''; auto. 
           - iApply (wp_bind (fill [SeqCtx])).
             iDestruct ((big_sepM_delete _ _ PC) with "Hmap") as "[HPC Hmap]"; [apply lookup_insert|].
             iApply (wp_notCorrectPC with "HPC"); [eapply not_isCorrectPC_perm; destruct p''; simpl in Hpft; try discriminate; eauto|].
@@ -74,9 +66,7 @@ Section fundamental.
             iNext. iIntros. discriminate. } }
       { rewrite lookup_insert_ne in HPC; auto.
         rewrite lookup_insert in HPC. inv HPC.
-        iDestruct (region_close with "[$Hstate $Hr $Ha $Hmono]") as "Hr"; eauto.
-        { destruct ρ;auto;[..|specialize (Hnotstatic g)];contradiction. }
-        iApply ("IH" $! _ (<[dst:=w0]> _) with "[%] [] [Hmap] [$Hr] [$Hsts] [$Hown]"); eauto.
+        iApply ("IH" $! (<[dst:=w0]> _) with "[%] [] [Hmap] [$Hown]"); eauto.
         - intros; simpl.
           rewrite lookup_insert_is_Some.
           destruct (reg_eq_dec dst x0); auto; right; split; auto.
@@ -90,13 +80,14 @@ Section fundamental.
             * destruct (reg_eq_dec PC r0).
               { subst r0.
                 - simplify_map_eq. 
-                  rewrite (fixpoint_interp1_eq _ (inr (_, g'', b'', e'', a''))) /=.
-                destruct Hp as [Hp | [Hp | [Hp Hg] ] ]; subst p''; try subst g'';
+                  rewrite !fixpoint_interp1_eq /=.
+                destruct Hp as [Hp | Hp]; subst p''; try subst g'';
                   (iFrame "Hinv Hexec"). }
               simplify_map_eq.
               iDestruct ("Hreg" $! r0 ltac:(auto)) as "Hr0". rewrite H0. auto.
           + repeat rewrite /RegLocate lookup_insert_ne; auto.
             iApply "Hreg"; auto.
+        - iAlways. rewrite !fixpoint_interp1_eq /=. destruct Hp as [-> | ->]; iFrame "Hinv".
       }
     }
     Unshelve. all: auto.
