theories/ftlr/ftlr_base.v
@@ -28,13 +28,14 @@ Section fundamental.
           -∗ na_own logrel_nais ⊤
           -∗ ⌜a1 = RX ∨ a1 = RWX⌝
              → □ (fixpoint interp1) (inr (a1, a2, a3, a4)) -∗ interp_conf)
+    -∗ (fixpoint interp1) (inr (p, b, e, a)) 
     -∗ inv (logN.@a) (∃ w0 : leibnizO Word, a ↦ₐ w0 ∗ P w0)
     -∗ (∀ r1 : RegName, ⌜r1 ≠ PC⌝ → (fixpoint interp1) (r !r! r1))
     -∗ ▷ □ (∀ w0 : Word, P w0 -∗ (fixpoint interp1) w0)
     -∗ na_own logrel_nais ⊤
     -∗ a ↦ₐ w
     -∗ ▷ P w
-    -∗ ▷ ((∃ w0 : leibnizO Word, a ↦ₐ w0 ∗ P w0) ={⊤ ∖ ↑logN.@a,⊤}=∗ emp)
+    -∗ (▷ (∃ w0 : leibnizO Word, a ↦ₐ w0 ∗ P w0) ={⊤ ∖ ↑logN.@a,⊤}=∗ emp)
     -∗ PC ↦ᵣ inr (p, b, e, a)
     -∗ ([∗ map] k↦y ∈ delete PC (<[PC:=inr (p, b, e, a)]> r), k ↦ᵣ y)
     -∗
