theories/fundamental.v
@@ -1,4 +1,4 @@
-(* From cap_machine.ftlr Require Export Jmp Jnz Get AddSubLt IsPtr Lea Load Mov Store Restrict Subseg LoadU StoreU PromoteU. *)
+From cap_machine.ftlr Require Export Jmp Jnz Mov Load. (* Jnz Get AddSubLt IsPtr Lea Load Mov Store Restrict Subseg LoadU StoreU PromoteU *)
 From iris.proofmode Require Import tactics.
 From iris.program_logic Require Import weakestpre adequacy lifting.
 From stdpp Require Import base.
@@ -64,16 +64,16 @@ Section fundamental.
         first apply (lookup_insert _ _ (inr (p, b, e, a))).
       destruct (decodeInstrW w) eqn:Hi. (* proof by cases on each instruction *)
       + (* Jmp *)
-        iApply (jmp_case with "[] [] [] [] [Hmono] [] [Hsts] [Hown] [Hr] [Hstate] [Ha] [HPC] [Hmap]");
+        iApply (jmp_case with "[] [] [] [] [] [Hown] [Ha] [HP] [Hcls] [HPC] [Hmap]");
           try iAssumption; eauto.
       + (* Jnz *)
-        iApply (jnz_case with "[] [] [] [] [Hmono] [] [Hsts] [Hown] [Hr] [Hstate] [Ha] [HPC] [Hmap]");
+        iApply (jnz_case with "[] [] [] [] [] [Hown] [Ha] [HP] [Hcls] [HPC] [Hmap]");
           try iAssumption; eauto.
       + (* Mov *)
-        iApply (mov_case with "[] [] [] [] [Hmono] [] [Hsts] [Hown] [Hr] [Hstate] [Ha] [HPC] [Hmap]");
+        iApply (mov_case with "[] [] [] [] [] [Hown] [Ha] [HP] [Hcls] [HPC] [Hmap]");
           try iAssumption; eauto.
       + (* Load *)
-        iApply (load_case with "[] [] [] [] [Hmono] [] [Hsts] [Hown] [Hr] [Hstate] [Ha] [HPC] [Hmap]");
+        iApply (load_case with "[] [] [] [] [] [Hown] [Ha] [HP] [Hcls] [HPC] [Hmap]");
           try iAssumption; eauto.
       + (* Store *)
         iApply (store_case with "[] [] [] [] [Hmono] [] [Hsts] [Hown] [Hr] [Hstate] [Ha] [HPC] [Hmap]");
